iris/UkFork.v
@@ -998,11 +998,10 @@ Section UkFork.
     rewrite (uexec_ret_ecall _ _ eq_refl).
     assert (Hnum : uvis_num (uvis_of_run m pc M pm sz fdv c gn Sc pidv false secc_all)
                    = USYS_fork).
-    { rewrite uvis_num_full0.
-      - cbn [uvis_tf uvis_of_run]. rewrite tf_of_num. exact Hn.
-      - reflexivity.
-      - cbn [uvis_tf uvis_of_run]. rewrite tf_of_num, Hn. usys_range. }
-    rewrite Hnum. cbv zeta.
+    { assert (Hraw : usys_num (uvis_tf (uvis_of_run m pc M pm sz fdv c gn Sc pidv false secc_all)) = USYS_fork)
+        by (cbn [uvis_tf uvis_of_run]; rewrite tf_of_num; exact Hn).
+      rewrite uvis_num_full0; [ exact Hraw | reflexivity | rewrite Hraw; usys_range ]. }
+    unfold uvis_num in Hnum. rewrite Hnum. cbv zeta.
     destruct (decide (USYS_fork = USYS_exit)) as [He | _];
       [ exfalso; unfold USYS_fork, USYS_exit in He; lia | ].
     destruct (decide (USYS_fork = USYS_fork)) as [_ | Hne];
